towards correctness

src/Util/FisherYates/Model.dfy
@@ -8,9 +8,11 @@ module FisherYates.Model {
   import Uniform
   import Rand
 
-  ghost function Shuffle<T>(xs: seq<T>, i: nat := 0): Monad.Hurd<seq<T>>
+  ghost function Shuffle<T>(xs: seq<T>, i: nat := 0): (h: Monad.Hurd<seq<T>>)
     requires i <= |xs|
     decreases |xs| - i
+    ensures forall s :: h(s).Result? ==> multiset(h(s).value) == multiset(xs)
+    ensures forall s :: h(s).Result? ==> |h(s).value| == |xs|
   {
     (s: Rand.Bitstream) =>
       if i < |xs| then
